theories/Syntax.v
@@ -499,7 +499,7 @@ with wf_proc : forall (m n:nat), lctxt m -> lctxt n -> proc -> Prop :=
     (r : rvar) (HR : r < n)
     (o : oper)
     (WFO : wf_oper m n G D o),
-    wf_proc m n G (D ⨥ (one n r)) (def r o)
+    wf_proc m n G ((one n r) ⨥ D) (def r o)
 
 | wf_app :
   forall m n
@@ -1553,9 +1553,6 @@ Proof.
     setoid_rewrite (ren_delta_compose _ (ren_id 1) 0 1 (wf_ren_id 1) (bij_ren_id 1)) in H; auto.
 Qed.    
 
-(* WIP ---------------------------------------------------------------------- *)
-(** FROM HERE DOWN IS WORK IN PROGRESS *)
-
 (* cuts *)
 
 (* "removes" variable x from the scope, where n is the number of variables > x *)
@@ -1586,24 +1583,38 @@ Definition cut_rvar_proc n x P : proc :=
 Definition retract_rvar_proc n x y P :=
   rename_rvar_proc (retract n x y) P.
 
-Import ListNotations.
-Fixpoint cuts n (l:list (nat * nat)) : ren (length l + n) n :=
-  match l with
-  | [] => ren_id n
-  | (x,y)::l =>
-      let f := cuts n l in
-      let x' := f x in
-      let y' := f y in
-          match Nat.compare x' y' with
-          | Lt => ren_compose f (retract n x' y')
-          | Eq => ren_compose f (cut n x')
-          | Gt => ren_compose f (retract n y' x')
-      end
-  end.
+
+(*
+Lemma wf_cut_oper :
+  forall m n x c o (G : lctxt m) (Dx : lctxt x) (Dn : lctxt n),
+    wf_oper m (x + 1 + n) G (Dx ⊗ 1[0 ↦ c] ⊗ Dn) o ->
+    wf_oper m (x + n) G (Dx ⊗ Dn) (cut_rvar_oper n x o).
+Proof.
+  intros.
+  inversion H; existT_eq; subst.
+  - simpl.
+*)
+
+
+
+
+(* Fixpoint cuts n (l:list (nat * nat)) : ren (length l + n) n := *)
+(*   match l with *)
+(*   | [] => ren_id n *)
+(*   | (x,y)::l => *)
+(*       let f := cuts n l in *)
+(*       let x' := f x in *)
+(*       let y' := f y in *)
+(*           match Nat.compare x' y' with *)
+(*           | Lt => ren_compose f (retract n x' y') *)
+(*           | Eq => ren_compose f (cut n x') *)
+(*           | Gt => ren_compose f (retract n y' x') *)
+(*       end *)
+(*   end. *)
 
 (* Operational Semantics --------------------------------------------------- *)
 
-
+Import ListNotations.
 Example ex_P0 : proc :=
   (par (def 3 (tup ([2])))
      (def 1 (tup ([4])))).
@@ -1615,26 +1626,47 @@ Example ex_P : proc :=
 
 Eval compute in retract_rvar_proc 1 1 3 ex_P0.
 
-Definition config := (nat * nat * proc)%type.
+(* (bag m n (par P (par (def r (tup rs1)) (def r (tup rs2))))) *)
+Inductive step_cuts : term -> term -> Prop :=
+| step_tup_nil :
+  forall m n P r,
+    step_cuts
+      (bag m (r + 1 + n) (par P (par (def r (tup nil)) (def r (tup nil)))))
+      (bag m (r + n) (cut_rvar_proc n r P))
 
-Definition step_cuts m n xs ys P : option config :=
-  let num_vars := length xs in 
-  if Nat.eq_dec num_vars (length ys) then
-    if lt_dec num_vars n then 
-      let cs := combine xs ys in
-      Some (m, (n-num_vars), rename_rvar_proc (cuts (n-num_vars) cs) P)
-    else
-      None
-  else
-    None.
+| step_tup_cons_l :
+  forall m n P r r1 r2 rs1 rs2 t'
+    (HLT: r1 < r2)
+    (HS: step_cuts (bag m (r2 + n)
+                  (retract_rvar_proc n r1 r2
+                     (par P (par (def r (tup rs1))
+                               (def r (tup rs2))))))
+               t'),
+    
+    (step_cuts (bag m (r2 + 1 + n) (par P (par (def r (tup (r1::rs1)))
+                                             (def r (tup (r2::rs2))))))
+       t')
 
-Eval compute in step_cuts 0 5 ([0;1;2]) ([0;3;4]) ex_P0.
+| step_tup_cons_r :
+  forall m n P r r1 r2 rs1 rs2 t'
+    (HLT: r2 < r1)
+    (HS: step_cuts (bag m (r1 + n)
+                  (retract_rvar_proc n r2 r1
+                     (par P (par (def r (tup rs1))
+                               (def r (tup rs2))))))
+               t'),
+    
+    (step_cuts (bag m (r1 + 1 + n) (par P (par (def r (tup (r1::rs1)))
+                                             (def r (tup (r2::rs2))))))
+       t').
 
 
-(*
-P |  r <- (x, y, z) | r <- (y, z, x)
-P {r=r}{x=y}{y=z}{z=x}
- *)
+
+      
+  
+
+
+
 
 Definition ren_f_extrude m m' : ren (m + m') (m' + m) :=
   fun x =>
@@ -1644,34 +1676,128 @@ Definition scope_extrude m m' n n' Q :=
     let Q1 := @rename_rvar_proc n (n' + n) (fun x => n + x) Q in
     let Q2 := @rename_fvar_proc (m + m') (m' + m) (ren_f_extrude m m') Q1 in
     Q2.
-    
-Inductive prim_step : config -> config -> Prop :=
+
+
+
+(*
+
+
+
+Inductive prim_step : term -> term -> Prop :=
 | step_tup_cut :
-  forall m n r rs1 rs2 P C,
-    step_cuts m n (r::rs1) (r::rs2) P = Some C ->
-    prim_step (m, n, par P (par (def r (tup rs1)) (def r (tup rs2))))
-      C
+  forall m n r rs1 rs2 P t,
+    step_cuts (r::rs1) (r::rs2) (bag m n P) = Some t ->
+    prim_step (bag m n (par P (par (def r (tup rs1)) (def r (tup rs2)))))
+      t
 
 | step_app :
   forall m m' n n' r r' f P Q,
     let Q' := retract_rvar_proc (m + m') r' m (scope_extrude m m' n n' Q) in
     prim_step
-      (m, n,
-        (par P
-        (par (def r (lam (bag m' n' Q)))
-        (par (def r (bng f))
-             (app f r')))))
-      (m' + m, n' + n,
-        (par P
-        (par (def r (lam (bag m' n' Q)))
-        (par (def r (bng f))
-           Q')))).
+      (bag m n
+         (par P
+         (par (def r (lam (bag m' n' Q)))
+         (par (def r (bng f))
+              (app f r')))))
+      (bag (m' + m) (n' + n)
+         (par P
+         (par (def r (lam (bag m' n' Q)))
+         (par (def r (bng f))
+              Q')))).
 
 Inductive  step : term -> term -> Prop :=
-| step_equiv : forall m n m' n' P P' Q,
-    P ≈p P' ->
-    prim_step (m, n, P') (m', n', Q) ->
-    step (bag m n P) (bag m' n' Q).
+| step_equiv : forall t1 t1' t2,
+    t1 ≈t t1' ->
+    prim_step t1' t2 ->
+    step t1 t2.
+
+Lemma wf_cuts :
+  forall m (G : lctxt m) rrs n (ls1 : list var) (ls2 : list var) (D : lctxt n) (D1 : lctxt n) P
+    (HLS: split rrs = (ls1, ls2))
+    (HLS1 : Forall (fun x => x < n) ls1)
+    (HLS2 : Forall (fun x => x < n) ls2)
+    (UD' : forall x, x < n -> D x = 2)
+    (HD : D1 ⨥ (SUM (map (one n) ls1) ⨥ SUM (map (one n) ls2)) = D)
+    (WFP : wf_proc m n G D1 P),
+  exists (D'' : lctxt (n - length rrs)),
+    (forall x, x < (n - length rrs) -> D'' x = 2) /\
+      wf_proc m (n - length rrs) G D'' (rename_rvar_proc (cuts (n - length rrs) rrs) P).
+Proof.
+  induction rrs; intros; simpl in *.
+  - inversion HLS; clear HLS.
+    subst. simpl in *.
+    exists D1.
+    split.
+    + rewrite sum_zero_r in UD'.
+      intros. apply UD'. lia.
+    + replace (n-0) with n by lia.
+      rewrite rename_rvar_id_proc with (m := m); auto.
+      apply tpo_wf_ws in WFP.
+      assumption.
+  - destruct a as [r1 r2].
+    destruct (split rrs).
+    inversion HLS; clear HLS.
+    rewrite <- H0 in HLS1.
+    inversion HLS1. subst. clear HLS1.
+    inversion HLS2; subst. clear HLS2.
+    assert (forall x : nat, x < n -> (D1 ⨥ (SUM (map (one n) l) ⨥ SUM (map (one n) l0))) x = 2).
+    { intros.
+      specialize (UD' x H).
+      simpl in UD'.
+      
+      
+    
+    
+*)    
+  
+  
+  
+
+(*
+
+(* Do we care only about stepping a top-level term? *)
+Lemma prim_step_wf :
+  forall m (G : lctxt m) (D : lctxt 0) (t t' : term)
+    (WF : wf_term m 0 G D t)
+    (STEP : prim_step t t'),
+    wf_term m 0 G D t'.
+Proof.
+  intros.
+  inversion STEP; subst; clear STEP.
+  - inversion WF; existT_eq; subst; clear WF.
+    inversion WFP; existT_eq; subst; clear WFP.
+    inversion WFP2; existT_eq; subst; clear WFP2.
+    inversion WFP0; existT_eq; subst; clear WFP0.
+    inversion WFP3; existT_eq; subst; clear WFP3.
+    inversion WFO; existT_eq; subst; clear WFO.
+    inversion WFO0; existT_eq; subst; clear WFO0.
+    rewrite sum_zero_r in H2.
+    subst.
+    replace (n + 0) with n in * by lia.
+    unfold step_cuts in H.
+    destruct (Nat.eq_dec (length (r::rs1)) (length (r::rs2))).
+    2 : { inversion H. }
+    assert ((one n r ⨥ SUM (map (one n) rs1)) = SUM (map (one n) (r::rs1))).
+    { reflexivity. }
+    rewrite H0 in H3; clear H0.
+    assert ((one n r ⨥ SUM (map (one n) rs2)) = SUM (map (one n) (r::rs2))).
+    { reflexivity. }
+    rewrite H0 in H3; clear H0.
+    remember (r :: rs1) as ls1.
+    remember (r :: rs2) as ls2.
+    remember (combine ls1 ls2) as rrs.
+    assert (split rrs = (ls1, ls2)).
+    { rewrite Heqrrs. apply combine_split; auto. }
+
+
+
+    
+    
+    
+    subst.
+    
+*)    
+
 
 
 
